theories/SLFCut.v
@@ -1,0 +1,123 @@
+(* ******************************************************* *)
+(** ** A simple yet non-structurally recursive definition of [wpgen] *)
+
+Module WPgenSubst.
+
+(** We are almost ready to formally define our function [wpgen].
+    There is one Coq-specific caveat on our way, however.
+    The definition of [wpgen] is not structurally recursive.
+    Thus, we'll have to play some tricks to first define it as a functional,
+    and then take the fixed point of this functional.
+
+    The details of this fixed point construction are not essential
+    for the moment; they are explained further in this chapter.
+    In any case, we will shortly afterwards present an alternative definition
+    to [wpgen] which is slightly more complex yet structurally recursive. *)
+
+Definition Wpgen wpgen (t:trm) : formula :=
+  mkstruct
+  match t with
+  | trm_val v =>
+       wpgen_val v
+  | trm_var x =>
+       wpgen_fail
+  | trm_fun x t1 =>
+       wpgen_val (val_fun x t1)
+  | trm_fix f x t1 =>
+       wpgen_val (val_fix f x t1)
+  | trm_app t1 t2 =>
+       wp t
+  | trm_seq t1 t2 =>
+       wpgen_seq (wpgen t1) (wpgen t2)
+  | trm_let x t1 t2 =>
+       wpgen_let (wpgen t1) (fun v => wpgen (subst x v t2))
+  | trm_if (trm_val v0) t1 t2 =>
+       wpgen_if v0 (wpgen t1) (wpgen t2)
+  | (* terms [trm_if t0 t1 t2] where [t0] is not a value or a variable
+       fall outside of the sub-language that we consider,
+       so let us here pretend that they are no such terms. *)
+    _ => wpgen_fail
+  end.
+
+(** To build the fixed point, we need to show the result type inhabited. *)
+
+Global Instance Inhab_formula : Inhab formula.
+Proof using. apply (Inhab_of_val (fun _ => \[])). Qed.
+
+(** [wpgen] is the fixed point of [Wpgen]. *)
+
+Definition wpgen := FixFun Wpgen.
+
+(** The fixed point equation, which enables unfolding the definition
+    of [wpgen], is proved further in this file. To establish it, we
+    essentially need to justify the termination of the recursive function. *)
+
+Parameter wpgen_fix : forall t,
+  wpgen t = Wpgen wpgen t.
+
+(** We establish the soundness of [wpgen] by induction on [t].
+    The induction principle that comes with the sublanguage
+    presented in [SLFRules] is as follows: *)
+
+Parameter trm_induct : forall (P : trm -> Prop),
+  (forall v, P (trm_val v)) ->
+  (forall x, P (trm_var x)) ->
+  (forall x t1 , P t1 -> P (trm_fun x t1)) ->
+  (forall (f:var) x t1, P t1 -> P (trm_fix f x t1)) ->
+  (forall t1, P t1 -> forall t2, P t2 -> P (trm_app t1 t2)) ->
+  (forall t1, P t1 -> forall t2, P t2 -> P (trm_seq t1 t2)) ->
+  (forall (x:var) t1, P t1 -> forall t2, P t2 -> P (trm_let x t1 t2)) ->
+  (forall t0, P t0 -> forall t1, P t1 -> forall t2, P t2 -> P (trm_if t0 t1 t2)) ->
+  (forall t, P t).
+
+(** However, it does not quite suite our needs. Indeed, in the case
+    of a [trm_let x t1 t2], the induction principle applies to [t2],
+    but we need to invoke it on [subst x v t2].
+
+    We thus exploit a variant induction principle, justified by an
+    induction on the size of a term, for a definition of size where
+    all values and functions are considered to be of size one unit.
+
+    This induction principle is stated below. The details of its proof
+    are not essential here; they may be found in the appendix to the
+    present chapter. *)
+
+Parameter trm_induct_subst : forall (P : trm -> Prop),
+  (forall v, P (trm_val v)) ->
+  (forall x, P (trm_var x)) ->
+  (forall x t1 , P (trm_fun x t1)) ->
+  (forall (f:var) x t1, P (trm_fix f x t1)) ->
+  (forall t1, P t1 -> forall t2, P t2 -> P (trm_app t1 t2)) ->
+  (forall t1, P t1 -> forall t2, P t2 -> P (trm_seq t1 t2)) ->
+  (forall (x:var) t1, P t1 -> forall t2, (forall v, P (subst x v t2)) -> P (trm_let x t1 t2)) ->
+  (forall t0, P t0 -> forall t1, P t1 -> forall t2, P t2 -> P (trm_if t0 t1 t2)) ->
+  (forall t, P t).
+
+(** The soundness lemma asserts: [forall t, formula_sound_for t (wpgen t)].
+    The proof is carried out by induction on [t]. For each term
+    construct, the proof consists of invoking the lemma [mkstruct_sound]
+    to justify soundness of the leading [mkstruct], then invoking
+    the soundness lemma specific to that term construct. *)
+
+Lemma wpgen_sound : forall t,
+  formula_sound_for t (wpgen t).
+Proof using.
+  intros. induction t using trm_induct_subst;
+   rewrite wpgen_fix; applys mkstruct_sound; simpl.
+  { applys wpgen_val_sound. }
+  { applys wpgen_fail_sound. }
+  { applys wpgen_fun_val_sound. }
+  { applys wpgen_fix_val_sound. }
+  { applys wp_sound. }
+  { applys wpgen_seq_sound. { applys IHt1. } { applys IHt2. } }
+  { applys wpgen_let_sound. { applys IHt1. } { intros v. applys H. } }
+  { destruct t1; try applys wpgen_fail_sound.
+    { applys wpgen_if_sound. { applys IHt2. } { applys IHt3. } } }
+Qed.
+
+Theorem triple_of_wpgen : forall t H Q,
+  H ==> wpgen t Q ->
+  triple t H Q.
+Proof using. introv M. rewrite wp_equiv. xchange M. applys wpgen_sound. Qed.
+
+End WPgenSubst.
